src/QueryConformance.v
@@ -120,5 +120,128 @@ Section QueryConformance.
     is_object_type schema n \/ is_interface_type schema n \/ is_union_type schema n.
   Proof.
   Admitted.
-  
+
+  Definition is_inline_fragment := @is_inline_fragment Name Vals.
+
+  Lemma union_type_lookup_union schema ty:
+    is_union_type schema ty ->
+    exists u mbs, lookup_type schema ty = Some (UnionTypeDefinition u mbs).
+  Proof.
+    rewrite /is_union_type.
+    case Hlook: lookup_type => [tdef|] //.
+    case: tdef Hlook => // u mbs. exists u. exists mbs. done.
+  Qed.
+    
+  Lemma nf_union_subqueries_inlines schema ty f α ϕ :
+    is_union_type schema f ->
+    query_conforms schema ty (NestedField f α ϕ) ->
+    all is_inline_fragment ϕ.
+  Proof.
+    move=> Hunion; move: (union_type_lookup_union Hunion).
+    case=> u; case=> mbs Hlook.
+    rewrite /query_conforms.
+    case Hlookf : lookup_field_in_type => [fld|] //.
+  Abort.
+
+  Lemma lookup_field_object_or_interface schema ty fname fld :
+    lookup_field_in_type schema ty fname = Some fld ->
+    is_object_type schema ty \/ is_interface_type schema ty.
+  Proof.
+    rewrite /lookup_field_in_type /fields.
+    case Hlook: lookup_type => [tdef|] //.
+    case: tdef Hlook => // [o intfs flds | i flds] Hlook _.
+    by left; rewrite /is_object_type Hlook.
+    by right; rewrite /is_interface_type Hlook.
+  Qed.
+
+  Lemma has_implementation_is_interface schema ty ty' :
+    ty' \in implementation schema ty ->
+            is_interface_type schema ty.
+  Proof.
+    rewrite /implementation.
+    case Hlook: lookup_type => [tdef|] //.
+    case: tdef Hlook => // i flds Hlook _.
+      by rewrite /is_interface_type Hlook.
+  Qed.
+
+  Lemma in_implementation_is_object schema ty :
+    forall ty', ty' \in implementation schema ty ->
+                   is_object_type schema ty'.
+    Admitted.
+
+  Lemma has_members_is_union schema ty ty' :
+    ty' \in union_members schema ty ->
+            is_union_type schema ty.
+  Proof.
+    rewrite /union_members.
+    case Hlook: lookup_type => [tdef|] //.
+    case: tdef Hlook => // i flds Hlook _.
+      by rewrite /is_union_type Hlook.
+  Qed.
+
+  Lemma in_union_is_object schema ty :
+    forall ty',
+      ty' \in union_members schema ty ->
+              is_object_type schema ty'.
+  Proof.
+    Admitted.
+            
+    
+  Lemma type_in_scope_N_scalar_enum schema type_in_scope ϕ :
+    query_conforms schema type_in_scope ϕ ->
+    [\/ is_object_type schema type_in_scope,
+     is_interface_type schema type_in_scope |
+     is_union_type schema type_in_scope].
+  Proof.
+    case: ϕ.
+    - move=> f α.
+      rewrite /query_conforms.
+      case Hlook: lookup_field_in_type => [fld|] // _.
+      move: (lookup_field_object_or_interface Hlook) => [Hobj | Hint].
+        by constructor 1.
+        by constructor 2.
+    - move=> l f α.
+      rewrite /query_conforms.
+      case Hlook: lookup_field_in_type => [fld|] // _.
+      move: (lookup_field_object_or_interface Hlook) => [Hobj | Hint].
+        by constructor 1.
+        by constructor 2.
+    - move=> f α ϕ.
+      rewrite /query_conforms.
+      case Hlook: lookup_field_in_type => [fld|] // _.
+      move: (lookup_field_object_or_interface Hlook) => [Hobj | Hint].
+        by constructor 1.
+        by constructor 2.
+    - move=> l f α ϕ.
+      rewrite /query_conforms.
+      case Hlook: lookup_field_in_type => [fld|] // _.
+      move: (lookup_field_object_or_interface Hlook) => [Hobj | Hint].
+        by constructor 1.
+        by constructor 2.
+    - move=> t ϕ.
+      rewrite /query_conforms.
+      case: ifP => //.
+      case: ifP => //.
+      move/or3P=> [/eqP -> | Himpl | Hunion].
+        by move=> Hobj _; constructor 1.
+        move: (has_implementation_is_interface Himpl) => Hint _ _.
+        by constructor 2.
+        move: (has_members_is_union Hunion).
+        by constructor 3.
+      case: ifP => //.
+      case: ifP => //.
+      move/orP=> [/eqP -> | Himpl].
+        by move=> Hint _ _; constructor 2.
+        move: (in_implementation_is_object Himpl) => Hobj _ _ _.
+        by constructor 1.
+      case: ifP => //.
+      case: ifP => /orP. move=> [/eqP -> | Hunion].
+        by move=> Hunion _ _ _; constructor 3.
+        rewrite -/query_conforms.
+        inversion schema.
+        move: (in_union_is_object Hunion) => Hobj _ _ _ _.
+          by constructor 1.
+          done.
+  Qed.
+      
 End QueryConformance.
